Blanc.lean
@@ -1,5 +1,6 @@
 import Lean.Data.Json
 import Lean.Data.Json.Parser
+import Lean.Data.HashSet
 import «Blanc».Weth
 
 
@@ -32,18 +33,7 @@ def WethByteCode : String :=
      "" <| List.map Bytes.toHexLine
         <| List.chunks 31 <| Option.getD weth.compile []
 
--- def main : IO Unit := IO.println WethByteCode
 
---mutual
---  inductive RLP : Type
---    | bytes : Bytes → RLP
---    | list : RLPs → RLP
---  inductive RLPs : Type
---    | nil : RLPs
---    | cons : RLP → RLPs → RLPs
---end
---
---#exit
 inductive RLP : Type
   | bytes : Bytes → RLP
   | list : List RLP → RLP
@@ -68,6 +58,18 @@ def Nat.toBytesCore (n : Nat) : Bytes :=
 
 def Nat.toBytes (n : Nat) : Bytes := n.toBytesCore.reverse
 
+def Nat.toBool : Nat → Bool
+  | 0 => 0
+  | _ => 1
+
+def Nat.toBitsAux' (n : Nat) : List Bool :=
+  if n < 2
+  then [n.toBool]
+  else (n % 2).toBool :: (n / 2).toBitsAux'
+
+def Nat.toBits' (m n : Nat) : Bits m :=
+  let bs := (List.takeD m (Nat.toBitsAux' n) 0).reverse
+  Bools.toBits m bs
 
 mutual
   def RLP.decode' : Nat → Bytes → Option (RLP × Bytes)
@@ -154,8 +156,6 @@ def Nibs.toBytes : List Nib → Option Bytes
 def Hex.toBytes (s : String) : Option Bytes :=
   s.data.mapM Hexit.toNib >>= Nibs.toBytes
 
-#eval (RLP.encode (.list [])).toHex
-
 def notTxBytes : Bytes :=
   (Hex.toBytes "f885800a8404c4b40094cccccccccccccccccccccccccccccccccccccccc01a4693c613900000000000000000000000000000000000000000000000000000000000000001ba0e8ff56322287185f6afd3422a825b47bf5c1a4ccf0dc0389cdc03f7c1c32b7eaa0776b02f9f5773238d3ff36b74a123f409cd6420908d7855bbe4c8ff63e00d698").getD []
 
@@ -179,6 +179,8 @@ def Bool.toByte : Bool → Byte
 
 def Byte.toUInt8 (b : Byte) : UInt8 := ⟨⟨b.toNat, b.toNat_lt_pow⟩⟩
 def UInt8.toByte (i : UInt8) : Byte := i.toBitVec.toFin.val.toByte
+def Bits.toUInt64 (xs : Bits 64) : UInt64 := ⟨⟨xs.toNat, xs.toNat_lt_pow⟩⟩
+def UInt64.toBits (i : UInt64) : Bits 64 := Nat.toBits 64 i.toBitVec.toFin.val
 
 def Bytes.toBytesArray (bs : Bytes) : ByteArray := ⟨⟨List.map Byte.toUInt8 bs⟩⟩
 def ByteArray.toBytes (a : ByteArray) : Bytes := a.data.toList.map UInt8.toByte
@@ -259,14 +261,17 @@ instance {ξ : Type u} [Ord ξ] : Ord (List ξ) := ⟨List.compare⟩
 abbrev NTB := Lean.RBMap Nibs Bytes compare
 abbrev Stor := Lean.RBMap Word Word compare
 
-structure PreAcct where
+structure EnvData where
+  (coinbase : Addr)
+
+structure PreData where
   (addr : Addr)
   (nonce : Bytes)
   (bal : Bytes)
   (stor : Stor)
   (code : Bytes)
 
-structure PostAcct where
+structure PostData where
   (hash : Word)
   (dataIdx : Nat)
   (gasIdx : Nat)
@@ -274,7 +279,7 @@ structure PostAcct where
   (logs : Word)
   (txdata : Bytes)
 
-structure TX : Type where
+structure TransactionData : Type where
   (data : List Bytes)
   (gasLimit : List Word)
   (gasPrice : Word)
@@ -284,26 +289,37 @@ structure TX : Type where
   (receiver : Addr)
   (value : List Word)
 
-structure TestFile where
+structure TestData where
   (info : Lean.Json)
-  (env  : Lean.Json)
-  (pre  : List PreAcct)
-  (post : String × List PostAcct)
-  (tx   : TX)
+  (env  : EnvData)
+  (pre  : List PreData)
+  (post : String × List PostData)
+  (tx   : TransactionData)
+
+structure Acct where
+  (nonce : Word)
+  (bal : Word)
+  (stor : Stor)
+  (code : Bytes)
+
+abbrev World' : Type := Lean.RBMap Addr Acct compare
 
 structure Test where
-  (pre  : List PreAcct)
+  (coinbase : Addr)
+  (world  : World')
   (txdata : Bytes)
-  (data : Bytes)
-  (gasLimit : Word)
-  (gasPrice : Word)
+
   (nonce : Word)
-  (secretKey : Word)
+  (gasPrice : Word)
+  (gasLimit : Word)
   (sender : Addr)
   (receiver : Addr)
   (value : Word)
+  (calldata : Bytes)
+
   (hash : Word) -- ?
   (logs : Word) -- keccak hash of (RLP-encoded) log items
+  (secret : Word)
 
 def pad : String → String
   | s => "  " ++ s
@@ -336,13 +352,37 @@ def encloseStrings : List String → List String
 def listToStrings {ξ} (f : ξ -> List String) (xs : List ξ) : List String :=
   encloseStrings (xs.map f).flatten
 
+def longBytesToStrings (hd : String) (bs : Bytes) : List String :=
+  match List.chunks 31 bs with
+  | [] => [hd]
+  | [bs'] => [s!"{hd} : {Bytes.toHex bs'}"]
+  | bss => "{hd} :" :: bss.map (λ bs' => pad (Bytes.toHex bs'))
+
 def txdataToStrings (tx : Bytes) : List String :=
   match List.chunks 31 tx with
   | [] => ["txdata :"]
   | [bs] => [s!"txdata : {Bytes.toHex bs}"]
   | bss => "txdata :" :: bss.map (λ bs => pad (Bytes.toHex bs))
 
-def postAcct.toStrings (p : PostAcct) : List String :=
+def Stor.toStrings (s : Stor) : List String :=
+  let kvs := s.toArray.toList
+  let kvToStrings : Word × Word → List String :=
+    λ nb => [s!"{nb.fst.toString} : {nb.snd.toString}"]
+  fork "stor" (kvs.map kvToStrings)
+
+  -- nonce : Word)
+  -- bal : Word)
+  -- stor : Stor)
+  -- code : Bytes)
+def Acct.toStrings (s : String) (a : Acct) : List String :=
+  fork s [
+    [s!"nonce : 0x{a.nonce.toHex 64}"],
+    [s!"bal : 0x{a.bal.toHex 64}"],
+    a.stor.toStrings,
+    longBytesToStrings "code" a.code
+  ]
+
+def postAcct.toStrings (p : PostData) : List String :=
   fork "Post Acct" [
     [s!"hash : {Bits.toHex 64 p.hash}"],
     [s!"data index : {p.dataIdx}"],
@@ -352,13 +392,16 @@ def postAcct.toStrings (p : PostAcct) : List String :=
     txdataToStrings p.txdata
   ]
 
-def Stor.toStrings (s : Stor) : List String :=
-  let kvs := s.toArray.toList
-  let kvToStrings : Word × Word → List String :=
-    λ nb => [s!"{nb.fst.toString} : {nb.snd.toString}"]
-  fork "stor" (kvs.map kvToStrings)
+def Lean.RBMap.toStrings {α β cmp} (m : Lean.RBMap α β cmp)
+  (fmt : α × β → List String): List String :=
+  let kvs := m.toArray.toList
+  fork "map" (kvs.map fmt)
 
-#check Bytes.toHex
+def World'.toStrings (w : World') : List String :=
+  let kvs := w.toArray.toList
+  let kvToStrings : Addr × Acct → List String :=
+    fun x => Acct.toStrings (x.fst.toHex 40) x.snd
+  fork "world" (kvs.map kvToStrings)
 
 def NTB.toStrings (s : NTB) : List String :=
   let kvs := s.toArray.toList
@@ -366,7 +409,7 @@ def NTB.toStrings (s : NTB) : List String :=
     λ nb => [s!"{nb.fst.toHex} : {nb.snd.toHex}"]
   fork "NTB" (kvs.map kvToStrings)
 
-def preAcct.toStrings (p : PreAcct) : List String :=
+def preAcct.toStrings (p : PreData) : List String :=
   fork "Pre Acct" [
     [s!"address : {Bits.toHex 40 p.addr}"],
     [s!"nonce : {Bytes.toHex p.nonce}"],
@@ -375,13 +418,18 @@ def preAcct.toStrings (p : PreAcct) : List String :=
     [s!"code : {Bytes.toHex p.code}"]
   ]
 
-def postToStrings : (String × List PostAcct) → List String
+def postToStrings : (String × List PostData) → List String
   | ⟨s, ps⟩ => fork "Post" [[s], listToStrings postAcct.toStrings ps]
 
-def preToStrings (l : List PreAcct) : List String :=
+def EnvData.toStrings (e : EnvData) : List String :=
+  fork "env" [
+    [s!"coinbase : {Bits.toHex 40 e.coinbase}"],
+  ]
+
+def preToStrings (l : List PreData) : List String :=
   fork "pre" [listToStrings preAcct.toStrings l]
 
-def TX.toStrings (tx : TX) : List String :=
+def TransactionData.toStrings (tx : TransactionData) : List String :=
   fork "transaction" [
     fork "data" [listToStrings (λ x => [Bytes.toHex x]) tx.data],
     fork "gasLimit" [listToStrings (λ x => [Bits.toHex 64 x]) tx.gasLimit],
@@ -393,16 +441,34 @@ def TX.toStrings (tx : TX) : List String :=
     fork "value" [listToStrings (λ x => [Bits.toHex 64 x]) tx.value]
   ]
 
-def TestFile.toStrings (t : TestFile) : List String :=
+def Test.toStrings (t : Test) : List String :=
+  fork "VM Test" [
+    [s!"coinbase : {t.coinbase.toHex 40}"],
+    t.world.toStrings,
+    txdataToStrings t.txdata,
+    [s!"nonce : 0x{t.nonce.toHex 64}"],
+    [s!"gas price : 0x{t.gasPrice.toHex 64}"],
+    [s!"gas limit : 0x{t.gasLimit.toHex 64}"],
+    [s!"sender : 0x{t.sender.toHex 40}"],
+    [s!"receiver : 0x{t.receiver.toHex 40}"],
+    [s!"value : 0x{t.value.toHex 64}"],
+    longBytesToStrings "calldata" t.calldata,
+    [s!"hash : 0x{t.hash.toHex 64}"],
+    [s!"logs : 0x{t.logs.toHex 64}"],
+    [s!"secret : 0x{t.secret.toHex 64}"]
+  ]
+
+def TestData.toStrings (t : TestData) : List String :=
   fork "VM Test" [
     ["info ..."],--t.info.toStrings,
-    ["env ..."],--t.env.toStrings,
+    EnvData.toStrings t.env,
     preToStrings t.pre,
     postToStrings t.post,
     t.tx.toStrings
   ]
 
-def TestFile.toString (t : TestFile) : String := Strings.join t.toStrings
+def TestData.toString (t : TestData) : String := Strings.join t.toStrings
+def Test.toString (t : Test) : String := Strings.join t.toStrings
 
 def IO.throw {ξ} (s : String) : IO ξ := MonadExcept.throw <| IO.Error.userError s
 
@@ -438,7 +504,7 @@ def Hex.from0x : String → IO String
   | ⟨'0' :: 'x' :: s⟩ => return ⟨s⟩
   | _ => IO.throw "prefix not 0x"
 
-def Lean.Json.toPostAcct : Json → IO PostAcct
+def Lean.Json.toPostData : Json → IO PostData
   | .obj r => do
     let hsx ← (r.find compare "hash").toIO "cannot retrieve hash bytes" >>= fromStr >>= Hex.from0x
     let hs ← (Hex.toBits 64 hsx).toIO "cannot convert hash bytes to word"
@@ -451,7 +517,7 @@ def Lean.Json.toPostAcct : Json → IO PostAcct
     let g ← (dgv.find compare "gas").toIO "cannot get gas" >>= Json.fromNum >>= JsonNumber.toNat
     let v ← (dgv.find compare "value").toIO "cannot get value" >>= Json.fromNum >>= JsonNumber.toNat
     return ⟨hs, d, g, v, lg, tx⟩
-  | _ => IO.throw "Json-to-PostAcct failed"
+  | _ => IO.throw "Json-to-PostData failed"
 
 
 -- def kbAdd {ξ υ o} (s : Lean.RBMap ξ υ o) (kv : (_ : String) × Json) : IO Stor := return s
@@ -465,33 +531,35 @@ def Lean.Json.toBits (n : Nat) (j : Json) : IO (Bits (4 * n)) := do
   (Hex.toBits n x).toIO ""
 
 
-def Lean.Json.toPreAcct (sj : (_ : String) × Json) : IO PreAcct := do
-  -- let a ← Hex.from0x sj.fst >>= (Option.toIO ∘ Hex.toBits 40)
+def Lean.Json.toPreData (sj : (_ : String) × Json) : IO PreData := do
   let ax ← Hex.from0x sj.fst
   let a ← (Hex.toBits 40 ax).toIO ""
   let r ← sj.snd.fromObj
-  let b ← ((r.find Ord.compare "balance").toIO "" >>= toBytes) --<&> Bytes.toBits 32
+  let b ← ((r.find Ord.compare "balance").toIO "" >>= toBytes)
   let c ← (r.find Ord.compare "code").toIO "" >>= toBytes
-  let n ← ((r.find Ord.compare "nonce").toIO "" >>= toBytes) -- <&> Bytes.toBits 32
-  --let sr ← (r.find Ord.compare "storage").toIO >>= fromObj
-  --let kvs := sr.toArray.toList
-  --let s ← kvs.foldlM Stor.add (Lean.RBMap.empty : Stor)
+  let n ← ((r.find Ord.compare "nonce").toIO "" >>= toBytes)
   return ⟨a, n, b, Lean.RBMap.empty, c⟩
 
-def Lean.Json.toPre (j : Lean.Json) : IO (List PreAcct) := do
+def Lean.Json.toEnvData (j : Lean.Json) : IO EnvData := do
+  let r ← j.fromObj
+  let cbj ← (r.find compare "currentCoinbase").toIO "No coinbase"
+  let bs ← cbj.toBytes
+  return ⟨bs.toBits 20⟩
+
+def Lean.Json.toPreDatas (j : Lean.Json) : IO (List PreData) := do
   let r ← j.fromObj
   let kvs := r.toArray.toList
-  mapM Lean.Json.toPreAcct kvs
+  mapM Lean.Json.toPreData kvs
 
-def Lean.Json.toPost (j : Lean.Json) : IO (String × List PostAcct) := do
+def Lean.Json.toPost (j : Lean.Json) : IO (String × List PostData) := do
   let ⟨k, j'⟩ ← j.fromSingleton
   let l ← j'.fromArr
-  let js ← mapM Lean.Json.toPostAcct l
+  let js ← mapM Lean.Json.toPostData l
   return ⟨k, js⟩
 
 def Bytes.toWord : Bytes → Word := Bytes.toBits 32
 
-def Lean.Json.toTX (j : Lean.Json) : IO TX := do
+def Lean.Json.toTransactionData (j : Lean.Json) : IO TransactionData := do
   let r ← j.fromObj
   let ds ← (r.find Ord.compare "data").toIO "" >>= fromArr >>= mapM toBytes
   let gls ← (r.find Ord.compare "gasLimit").toIO "" >>= fromArr >>= mapM toBytes
@@ -503,55 +571,55 @@ def Lean.Json.toTX (j : Lean.Json) : IO TX := do
   let vs ← (r.find Ord.compare "value").toIO "" >>= fromArr >>= mapM toBytes
   return ⟨ds, gls.map Bytes.toWord, gp, n, sk, sd, rc, vs.map Bytes.toWord⟩
 
-def Lean.Json.toTestFile (j : Lean.Json) : IO TestFile := do
+def Lean.Json.toTestData (j : Lean.Json) : IO TestData := do
   let (_, .obj r) ← j.fromSingleton | IO.throw "not singleton object"
   let info ← (r.find compare "_info").toIO ""
-  let env ←  (r.find compare "env").toIO ""
-  let pre ←  (r.find compare "pre").toIO "" >>= Lean.Json.toPre
+  let env ←  (r.find compare "env").toIO "" >>= Lean.Json.toEnvData
+  let pre ←  (r.find compare "pre").toIO "" >>= Lean.Json.toPreDatas
   let post ← (r.find compare "post").toIO "" >>= Lean.Json.toPost
-  let tx ←   (r.find compare "transaction").toIO "" >>= Lean.Json.toTX
+  let tx ←   (r.find compare "transaction").toIO "" >>= Lean.Json.toTransactionData
   return ⟨info, env, pre, post, tx⟩
 
--- structure PostAcct where
---   (hash : Word)
---   (dataIdx : Nat)
---   (gasIdx : Nat)
---   (valueIdx : Nat)
---   (logs : Word)
---   (txdata : Bytes)
---
--- structure TX : Type where
---   (data : List Bytes)
---   (gasLimit : List Word)
---   (gasPrice : Word)
---   (nonce : Word)
---   (secretKey : Word)
---   (sender : Addr)
---   (receiver : Addr)
---   (value : List Word)
 
-def getTest (ps : List PreAcct) (tx : TX) (p : PostAcct) : IO Test := do
-  let d ← (List.get? tx.data p.dataIdx).toIO ""
-  let gl ← (List.get? tx.gasLimit p.gasIdx).toIO ""
-  let vl ← (List.get? tx.value p.valueIdx).toIO ""
+
+def TestData.world (td : TestData) : World' :=
+  let aux : PreData → (Addr × Acct) :=
+    fun pd => ⟨
+      pd.addr,
+      {
+        nonce := pd.nonce.toBits 32,
+        bal := pd.bal.toBits 32
+        stor := pd.stor
+        code := pd.code
+      }
+    ⟩
+  Lean.RBMap.fromList (td.pre.map aux) _
+
+def getTest (td : TestData) (p : PostData) : IO Test := do
+  let cd ← (List.get? td.tx.data p.dataIdx).toIO ""
+  let gl ← (List.get? td.tx.gasLimit p.gasIdx).toIO ""
+  let vl ← (List.get? td.tx.value p.valueIdx).toIO ""
   return {
-    pre := ps
+    coinbase := td.env.coinbase
+    world := td.world
     txdata := p.txdata
-    data := d
+    calldata := cd
     gasLimit := gl
-    gasPrice := tx.gasPrice
-    nonce := tx.nonce
-    secretKey := tx.secretKey
-    sender := tx.sender
-    receiver := tx.receiver
+    gasPrice := td.tx.gasPrice
+    nonce := td.tx.nonce
+    secret := td.tx.secretKey
+    sender := td.tx.sender
+    receiver := td.tx.receiver
     value := vl
     hash := p.hash
     logs := p.logs
   }
 
-def getTests (t : TestFile) : IO (List Test) := do
+
+
+def getTests (t : TestData) : IO (List Test) := do
   have ps := t.post.snd
-  mapM (getTest t.pre t.tx) ps
+  mapM (getTest t) ps
 
 def Lean.RBMap.fromSingleton {ξ υ f} (m : RBMap ξ υ f) : Option (ξ × υ) :=
   match m.toList with
@@ -698,7 +766,7 @@ def Stor.toNTB (s : Stor) : NTB :=
         (RLP.encode <| .bytes <| @Bits.toBytes 32 v)
   Lean.RBMap.fold f NTB.empty s
 
-def PreAcct.toKV (a : PreAcct) : Nibs × Bytes :=
+def PreData.toKV (a : PreData) : Nibs × Bytes :=
   ⟨
     @Bits.toNibs 64 (@Bits.toBytes 20 a.addr).keccak,
     RLP.encode <| .list [
@@ -709,53 +777,6 @@ def PreAcct.toKV (a : PreAcct) : Nibs × Bytes :=
     ]
   ⟩
 
-def testStor : Stor :=
-  Lean.RBMap.singleton 0
-    ((Hex.toWord "fffffffffffffffffffffffffffffffffffffffffffffffffedcba9876543210").getD 0)
-
-def testPreAcct1 : PreAcct :=
-  {
-    addr := (Hex.toBits 40 "0000000000000000000000000000000000001000").getD 0
-    nonce := []
-    bal := (Hex.toBytes "0ba1a9ce0ba1a9ce").getD []
-    stor := testStor
-    code := (Hex.toBytes "670123456789abcdef1960005500").getD []
-  }
-
-def testPreAcct2 : PreAcct :=
-  {
-    addr := (Hex.toBits 40 "a94f5374fce5edbc8e2a8697c15331677e6ebf0b").getD 0
-    nonce := [Ox x0 x1]
-    bal := (Hex.toBytes "0ba1a9ce0b9aa79f").getD []
-    stor := .empty
-    code := []
-  }
-
-def testPreAcct3 : PreAcct :=
-  {
-    addr := (Hex.toBits 40 "cccccccccccccccccccccccccccccccccccccccc").getD 0
-    nonce := []
-    bal := (Hex.toBytes "0ba1a9ce0ba1a9cf").getD []
-    stor := .empty
-    code := (Hex.toBytes "600060006000600060006004356110000162fffffff100").getD []
-  }
-
-def testPreAccts : List PreAcct := [testPreAcct1, testPreAcct2, testPreAcct3]
-
-def testNTB : NTB := Lean.RBMap.fromList (List.map PreAcct.toKV testPreAccts) compare
-
--- def main : IO Unit := do IO.println <| Bits.toHex 64 (trie testNTB)
-
--- def main : IO Unit := do
---   let t ← readJsonFile "not.json" >>= Lean.Json.toTestFile
---   IO.println t.toString
-
-def callData : Bytes :=
-  (Hex.toBytes "693c6139").getD []
-
-def dataGas (cd : Bytes) : Nat :=
-  let aux : Byte → Nat := fun b => if b = 0 then 4 else 16
-  (cd.map aux).sum
 
 def G_initcodeword : Nat := 2
 
@@ -766,97 +787,766 @@ def G_txcreate : Nat := 32000
 def G_accesslistaddress : Nat := 2400
 def G_accessliststorage : Nat := 1900
 
-def intrinsicGas (Tt : Bytes) (cd : Bytes) (Ta : List (Addr × List Word)) : Nat :=
-  let aux : (Addr × List Word) → Nat :=
-    fun | ⟨_, l⟩ => G_accesslistaddress + (G_accessliststorage * l.length)
-  dataGas cd +
-  (if Tt = [] then G_txcreate + initCodeCost cd else 0) +
-  2100 +
-  (Ta.map aux).sum
 
-def Tg : Nat := ((Hex.toBytes "04C4B400").getD []).toNat
 
-def g : Nat := Tg - intrinsicGas ((Hex.toBytes "cccccccccccccccccccccccccccccccccccccccc").getD []) callData []
 
-def C : Nat := _ + _
+instance : Hashable Addr := ⟨Bits.toUInt64 ∘ @Bits.suffix 64 96⟩
+instance : Hashable (Addr × Word) := ⟨Bits.toUInt64 ∘ @Bits.suffix 64 96 ∘ Prod.fst⟩
 
-def g' : Nat := g - C
+abbrev AddrSet : Type := @Std.HashSet Addr _ _ --⟨Bits.toUInt64 ∘ @Bits.suffix 64 96⟩
+abbrev StorKeySet : Type := @Std.HashSet (Addr × Word) _ _
 
-structure Acct where
-  (nonce : Word)
-  (bal : Word)
-  (stor : Stor)
-  (code : Bytes)
+structure Accrual where
+  (dest : List Addr) -- A_s
+  (adrs : AddrSet) -- A_s
+  (keys : StorKeySet) -- A_k
+  (ref : Nat) -- A_r
+  -- (sac : Nat) -- A_r
 
-abbrev World' : Type := Lean.RBMap Addr Acct compare
+structure Machine where
+  (gas : Nat) -- μ_g
+  (pc : Nat) -- μ_pc
+  (mem : Bytes) -- μ_m
+  (ret : Bytes) -- μ_o
+  (stk : Stack) -- μ_s
+
+def ceilDiv (m n : Nat) := m / n + if m % n = 0 then 0 else 1
+
+-- μ_i : no need to make it a separate field of Machine,
+-- when it is completely determined by Machine.mem
+def Machine.msz (m : Machine) : Nat := ceilDiv m.mem.length 32
+
+structure Block where
+  (ben : Addr) -- H_c
+
+structure Env' where
+  (cta : Addr) -- contract address (YP : a)
+  (oga : Addr) -- origin address (YP : o)
+  (gpr : Word) -- gas price (YP : p)
+  (cld : Bytes) -- calldata (YP : d)
+  (cla : Addr) -- caller Addr (YP : s)
+  (clv : Word) -- callvalue (YP : v)
+  (code : Bytes) -- contract code  (YP : b)
+  (blk : Block) -- block (YP : H)
+  (exd : Nat) -- execution depth (YP : e)
+  (wup : Bool) -- World-State update permission (YP : w)
 
 structure State' where
-  (w : World')
-  (cta : Addr)
-  (pc : Nat)
+  (wld : World')
+  (mcn : Machine)
+  (acr : Accrual)
+  (env : Env')
 
-def testWorld : World' :=
-  let aux : PreAcct → (Addr × Acct) :=
-    fun pa => ⟨pa.addr, ⟨pa.nonce.toBits 32, pa.bal.toBits 32, pa.stor, pa.code⟩⟩
-  Lean.RBMap.fromList (testPreAccts.map aux) _
+structure Ξ.Result where
+  (wld : Option World')
+  (gas : Nat)
+  (acr : Accrual)
+  (ret : Option Bytes)
 
-def testState : State' :=
-  {
-    w := testWorld
-    cta := (Hex.toBits 40 "cccccccccccccccccccccccccccccccccccccccc").getD 0
-    pc := 0
+structure exec.Result where
+  (wld : Option World')
+  (mcn : Machine)
+  (acr : Accrual)
+  (ret : Option Bytes)
+
+inductive Inst : Type
+  | last : Linst → Inst
+  | next : Ninst → Inst
+  | jump : Jinst → Inst
+
+lemma List.length_takeD {ξ : Type u} (n : Nat) (xs : List ξ) (x : ξ) :
+    (List.takeD n xs x).length = n := by
+  induction n with
+  | zero => rfl
+  | succ n ih => simp [takeD]
+
+def State'.inst (s : State') : Option Inst := do
+  let a ← s.wld.find? s.env.cta
+  match a.code.get? s.mcn.pc with
+  | none => return (.last .stop)
+  | some b =>
+    (b.toRinst? <&> (.next ∘ .reg)) <|>
+    (b.toXinst? <&> (.next ∘ .exec)) <|>
+    (b.toJinst? <&> .jump) <|>
+    (b.toLinst? <&> .last) <|>
+    ( if h : 95 ≤ b.toNat ∧ b.toNat ≤ 127
+      then let len := b.toNat - 95
+           let slc := a.code.sliceD (s.mcn.pc + 1) len 0
+           let h_slc : slc.length ≤ 32 := by
+             simp [len, slc, List.sliceD, h.right]
+           some (.next <| .push slc h_slc)
+      else none )
+
+def g_zero : Nat := 0
+def g_verylow : Nat := 3
+
+def safeSub {ξ} [Sub ξ] [LE ξ] [@DecidableRel ξ (· ≤ ·)] (x y : ξ) : Option ξ :=
+  if y ≤ x then some (x - y) else none
+
+def State'.deductGas (s : State') (c : Nat) : Option Nat := safeSub s.mcn.gas c
+
+def Rinst.run (s : State') : Rinst → Option State'
+  | .add => do
+    let (x :: y :: xs) ← (return s.mcn.stk) | none
+    let g' ← safeSub s.mcn.gas g_verylow
+    return {s with mcn := {s.mcn with stk := (x + y) :: xs, gas := g', pc := s.mcn.pc + 1}}
+  | .calldataload => do
+    let (x :: xs) ← (return s.mcn.stk) | none
+    let g' ← s.deductGas g_verylow
+    let cd : Word := Bytes.toBits 32 (s.env.cld.sliceD x.toNat 32 0)
+    return {s with mcn := {s.mcn with stk := cd :: xs, gas := g', pc := s.mcn.pc + 1}}
+  | _ => none
+
+def Acct.Empty (a : Acct) : Prop :=
+  a.code = [] ∧ a.nonce = 0 ∧ a.bal = 0
+
+def Dead (w : World') (a : Addr) : Prop :=
+  match w.find? a with
+  | none => True
+  | some x => x.Empty
+
+def gNewAccount : Nat := 25000
+def gCallValue : Nat := 9000
+def gCallStipend : Nat := 2300
+
+instance {w a} : Decidable (Dead w a) := by
+  simp [Dead]
+  cases (Lean.RBMap.find? w a)
+  · simp; apply instDecidableTrue
+  · simp [Acct.Empty]; apply instDecidableAnd
+
+def gWarmAccess : Nat := 100
+def gColdAccountAccess : Nat := 2600
+
+def cAAccess (x : Addr) (a : AddrSet) : Nat :=
+  if x ∈ a then gWarmAccess else gColdAccountAccess
+
+def except64th (n : Nat) : Nat := n - (n / 64)
+
+def cExtra (s : State') (t : Addr) (v : Word) : Nat :=
+  let cNew : Nat := if (Dead s.wld t ∧ v ≠ 0) then gNewAccount else 0
+  let cXfer : Nat := if v ≠ 0 then gCallValue else 0
+  cAAccess t s.acr.adrs + cXfer + cNew
+
+def cGasCap (s : State') (g : Nat) (t : Addr) (v : Word) : Nat :=
+    if cExtra s t v ≤ s.mcn.gas
+    then min (except64th (s.mcn.gas - cExtra s t v)) g
+    else g
+
+def cCallGas (s : State') (g : Nat) (t : Addr) (v : Word) : Nat :=
+  if v ≠ 0
+  then cGasCap s g t v + gCallStipend
+  else cGasCap s g t v
+
+def cCall (s : State') (g : Nat) (t : Addr) (v : Word) : Nat :=
+  cGasCap s g t v + cExtra s t v
+
+structure theta.Result : Type where
+  (wld : World')
+  (gas : Nat)
+  (acr : Accrual)
+  (sta : Word)
+  (ret : Bytes)
+
+def World'.code (w : World') (a : Addr) : Bytes :=
+  match w.find? a with
+  | none => []
+  | some x => x.code
+
+-- need further update for precompiled contracts
+def θ.prep
+  (H : Block)
+  (σ : World')
+  (A : Accrual)
+  (s : Addr)
+  (o : Addr)
+  (r : Addr)
+  (c : Addr)
+  (g : Nat)
+  (p : Nat)
+  (v : Word)
+  (v_app : Word)
+  (d : Bytes)
+  (e : Nat)
+  (w : Bool) :
+  State' :=
+  let σ'₁ : World' :=
+    match σ.find? r with
+    | none =>
+      if v = 0
+      then σ
+      else σ.insert r {nonce := 0, bal := v, stor := .empty, code := []}
+    | some aᵣ => σ.insert r {aᵣ with bal := aᵣ.bal + v}
+  let σ₁ : World' :=
+    match σ'₁.find? s with
+    | none =>
+      if v = 0
+      then σ'₁
+      else (dbg_trace "unreachable code : nonzero value calls from empty accounts should never happen" ; σ'₁)
+    | some aₛ => σ.insert s {aₛ with bal := aₛ.bal - v}
+  let cd : Bytes := σ.code c
+  let I : Env' := {
+    cta := r, oga := o, gpr := @Nat.toBits 256 p, cld := d
+    cla := s, clv := v_app, code := cd, blk := H, exd := e, wup := w
   }
+  let μ : Machine := {gas := g, pc := 0, mem := [], ret := [], stk := []}
+  ⟨σ₁, μ, A, I⟩
 
-def State'.inst (s : State') : IO (Inst ⊕ Hinst) := do
-  let a ← (s.w.find? s.cta).toIO "contract does not exist in state"
-  match a.code.get? s.pc with
-  | none =>
-    if a.code.length = s.pc
-    then return (.inr .stop)
-    else .throw "unreachable code : out-of-bound instruction lookup inconsistent with normal usage"
-  | some b => _
+def θ.wrap (s : State') (oxr : Option exec.Result) : theta.Result :=
+  let xr : exec.Result := oxr.getD ⟨none, s.mcn, s.acr, none⟩
+  let Ξr : Ξ.Result := {wld := xr.wld, gas := xr.mcn.gas, acr := xr.acr, ret := xr.ret}
+  let σ_stars : Option World' := Ξr.wld
+  let g_stars : Nat := Ξr.gas
+  let A_stars : Accrual := Ξr.acr
+  let o : Option Bytes := Ξr.ret
 
-#exit
+  let σ' : World' := σ_stars.getD s.wld
+  let g' : Nat := if σ_stars.isNone ∧ o.isNone then 0 else g_stars
+  let A' : Accrual := if σ_stars.isNone then s.acr else A_stars
+  let z : Word := if σ_stars.isNone then 0 else 1
 
-def State'.gas (s : State') : IO Nat := do
-  let a ← (s.w.find? s.cta).toIO "cannot get acct"
-  let c ← (a.code.get? s.pc).toIO "cannot"
+  -- o' is not from YP, but necessary to cast from 'Option Bytes' to 'Bytes'
+  -- (YP is a bit sloppy with types here)
+  let o' : Bytes := o.getD []
+  ⟨σ', g', A', z, o'⟩
 
-  _
 
+-- returns 'none' IFF either
+-- (1) VM is CURRENTLY at EHS, due to the code byte at PC (not at some later point in code), or
+-- (2) recursion limit is reached (should never happen with correct usage)
+def execAux (s s' : State') (f : State' → Option exec.Result) : exec.Result :=
+  let g' : Nat := s'.mcn.gas
+  let s'' := {s' with mcn := {s'.mcn with gas := g'}}
+  (f s'').getD ⟨none, s''.mcn, s''.acr, none⟩
 
-#exit
+def gColdSLoad : Nat := 2100
+def gSSet : Nat := 20000
+def gSReset : Nat := 2900
+def rSClear : Nat := 4800
 
+def Jinst.toString : Jinst → String
+  | .jump => "JUMP"
+  | .jumpdest => "JUMPDEST"
+  | .jumpi => "JUMPI"
+
+def Inst.toString : Inst → String
+  | .next n => n.toString
+  | .jump j => j.toString
+  | .last l => l.toString
 
 def Bits.min {n} : Bits n → Bits n → Bits n
   | xs, ys => if xs ≤ ys then xs else ys
 
 instance {n} : Min (Bits n) := ⟨.min⟩
 
-def A_r : Word := 0 -- SSTORE used only once, cannot change from 0
+def testStor : Stor :=
+  Lean.RBMap.singleton 0
+    ((Hex.toWord "fffffffffffffffffffffffffffffffffffffffffffffffffedcba9876543210").getD 0)
 
-def gstar : Word := g' + min ((Tg - gprime) / 5) A_r
+def testerAdr : Addr := (Hex.toBits 40 "0000000000000000000000000000000000001000").getD 0
+def senderAdr : Addr := (Hex.toBits 40 "a94f5374fce5edbc8e2a8697c15331677e6ebf0b").getD 0
+def receiverAdr : Addr := (Hex.toBits 40 "cccccccccccccccccccccccccccccccccccccccc").getD 0
 
-def balInit : Word := Bytes.toWord ((Hex.toBytes "0ba1a9ce0ba1a9ce").getD [])
+def beforeBal : Word := Bytes.toBits 32 <| (Hex.toBytes "0ba1a9ce0ba1a9ce").getD []
 
-def txVal : Word := 1
 
-def Yg : Word := Tg - gstar
+def beforeTesterAcct : Acct :=
+  {
+    nonce := 0
+    bal := beforeBal
+    stor := .empty
+    code := (Hex.toBytes "670123456789abcdef1960005500").getD []
+  }
 
-def gasPrice : Word := 10--Bytes.toWord ((Hex.toBytes "0a").getD [])
+def afterTesterAcct : PreData :=
+  {
+    addr := testerAdr
+    nonce := []
+    bal := (Hex.toBytes "0ba1a9ce0ba1a9ce").getD []
+    stor := testStor
+    code := (Hex.toBytes "670123456789abcdef1960005500").getD []
+  }
 
-def balFinal : Word := balInit - ((Yg * gasPrice) + txVal)
+def beforeSenderAcct : Acct :=
+  {
+    nonce := 0
+    bal := beforeBal
+    stor := .empty
+    code := []
+  }
+
+def afterSenderAcct : PreData :=
+  {
+    addr := senderAdr
+    nonce := [Ox x0 x1]
+    bal := (Hex.toBytes "0ba1a9ce0b9aa79f").getD []
+    stor := .empty
+    code := []
+  }
+
+def beforeReceiverAcct : Acct :=
+  {
+    nonce := 0
+    bal := beforeBal
+    stor := .empty
+    code := (Hex.toBytes "600060006000600060006004356110000162fffffff100").getD []
+  }
+
+def afterReceiverAcct : PreData :=
+  {
+    addr := receiverAdr
+    nonce := []
+    bal := (Hex.toBytes "0ba1a9ce0ba1a9cf").getD []
+    stor := .empty
+    code := (Hex.toBytes "600060006000600060006004356110000162fffffff100").getD []
+  }
+
+def afterPreDatas : List PreData :=
+  [
+    afterTesterAcct,
+    afterSenderAcct,
+    afterReceiverAcct
+  ]
+
+def testNTB : NTB := Lean.RBMap.fromList (List.map PreData.toKV afterPreDatas) compare
+
+
+def beforeWorld : World' :=
+  Lean.RBMap.fromList
+    [
+      ⟨testerAdr, beforeTesterAcct⟩,
+      ⟨senderAdr, beforeSenderAcct⟩,
+      ⟨receiverAdr, beforeReceiverAcct⟩
+    ]
+    _
+
+def afterWorld : World' :=
+  let aux : PreData → (Addr × Acct) :=
+    fun pa => ⟨pa.addr, ⟨pa.nonce.toBits 32, pa.bal.toBits 32, pa.stor, pa.code⟩⟩
+  Lean.RBMap.fromList (afterPreDatas.map aux) _
+
+
+-- gas limit ('T_g' in YP)
+def Tg : Nat := ((Hex.toBytes "04C4B400").getD []).toNat
+def testGasLimit : Nat := ((Hex.toBytes "04C4B400").getD []).toNat
+
+def dataGas (cd : Bytes) : Nat :=
+  let aux : Byte → Nat := fun b => if b = 0 then 4 else 16
+  (cd.map aux).sum
+
+def gTransaction : Nat := 21000
+
+def intrinsicGas (Rcv : Option Addr) (cd : Bytes) (Ta : List (Addr × List Word)) : Nat :=
+  let aux : (Addr × List Word) → Nat :=
+    fun | ⟨_, l⟩ => G_accesslistaddress + (G_accessliststorage * l.length)
+  dataGas cd +
+  Rcv.rec (G_txcreate + initCodeCost cd) (fun _ => 0) +
+  gTransaction +
+  (Ta.map aux).sum
+
+def testCallData : Bytes :=
+  (Hex.toBytes "693c61390000000000000000000000000000000000000000000000000000000000000000").getD []
+
+def g₀ : Nat := intrinsicGas (some receiverAdr) testCallData []
+
+def g : Nat := Tg - g₀
+
+
+def World'.transfer? (wld : World') (src : Addr) (clv : Word) (dst : Addr) : Option World' := do
+  let src_acct ← wld.find? src
+  let dst_acct ← wld.find? dst
+  let new_src_bal ← safeSub src_acct.bal clv
+  let wor' := wld.insert src {src_acct with bal := new_src_bal}
+  return wor'.insert dst {dst_acct with bal := dst_acct.bal + clv}
+
+-- checkpoint is an 'Option' type because computation of checkpoints
+-- may fail for invalid txs. this is *not* the case for any subsequent
+-- steps of a tx: once you get to a checkpoint, the tx *always* goes
+-- through and yields a new state. i.e., there is no invalid tx that
+-- has a checkpoint.
+def checkpoint (w : World') (ad : Addr) (v : Word) : Option World' := do
+  let ac ← w.find? ad
+  let bal' ← safeSub ac.bal v
+  some <| w.insert ad {ac with bal := bal', nonce := ac.nonce + 1}
+
+def testCoinbase : Addr := (Hex.toBits 40 "2adc25665018aa1fe0e6bc666dac8fc2697ff9ba").getD 0
+
+def testCheckpoint : World' := (checkpoint beforeWorld senderAdr 1).getD beforeWorld
+
+-- A^0
+def Accrual.init : Accrual :=
+  {
+    dest := []
+    adrs := Std.HashSet.ofList [1, 2, 3, 4, 5, 6, 7, 8, 9]
+    keys := .empty
+    ref := 0
+  }
+
+abbrev AccessList : Type := List (Addr × List Word)
+
+abbrev AccessList.collect (al : AccessList) : StorKeySet :=
+  let addPair : Addr → StorKeySet → Word → StorKeySet :=
+    fun a aks k => aks.insert ⟨a, k⟩
+  let addElem : StorKeySet → Addr × List Word → StorKeySet :=
+    fun aks pr => List.foldl (addPair pr.fst) aks pr.snd
+  List.foldl addElem .empty al
+
+def A_star (H : Block) (ST : Addr) (Tt : Option Addr) (TA : AccessList) : Accrual :=
+  let a : AddrSet :=
+    Accrual.init.adrs.insertMany
+      (Std.HashSet.ofList (ST :: H.ben :: TA.map Prod.fst))
+  {
+    Accrual.init with
+    adrs := Tt.rec a (a.insert)
+    keys := TA.collect
+  }
+
+def testBlock : Block := {ben := testCoinbase}
+
+def sstoreStep (w₀ : World') (s : State') : Option State' := do
+  let ⟨σ, μ, A, I⟩ := s
+  let (x :: v' :: xs) ← (return μ.stk) | none
+  let (a₀ : Acct) ← w₀.find? I.cta
+  let (v₀ : Word) := (a₀.stor.find? x).getD 0
+  let (a : Acct) ← σ.find? s.env.cta
+  let (v : Word) := (a.stor.find? x).getD 0
+  let c₀ : Nat := cond (A.keys.contains ⟨I.cta, x⟩) 0 gColdSLoad
+  -- let .true ← (dbg_trace s!"v₀ : {Bits.toHex 64 v₀}\nv : {Bits.toHex 64 v}\nv' : {Bits.toHex 64 v'}"; return true) | none
+  let c₁ : Nat :=
+    if v = v' ∨ v₀ ≠ v
+    then gWarmAccess
+    else if v₀ = 0
+         then gSSet
+         else gSReset
+  let c : Nat := c₀ + c₁
+  let rDirtyClear : Int :=
+    if v₀ ≠ 0 ∧ v = 0
+    then (- rSClear)
+    else if v₀ ≠ 0 ∧ v' = 0
+         then rSClear
+         else 0
+  let rDirtyReset : Int :=
+    if v₀ = v'
+    then if v₀ = 0
+         then gSSet - gWarmAccess
+         else gSReset - gWarmAccess
+    else 0
+  let r : Int :=
+    if v = v'
+    then 0
+    else if v₀ = v
+         then if v₀ = 0
+              then rSClear
+              else 0
+         else rDirtyClear + rDirtyReset
+  let g' ← safeSub s.mcn.gas c
+  let ref' ← (Int.ofNat A.ref + r).toNat'
+  let a' : Acct := {a with stor := a.stor.insert x v'}
+
+  some
+    {
+      wld := σ.insert I.cta a'
+      mcn := {
+        s.mcn with
+        gas := g'
+        pc := s.mcn.pc + 1
+        stk := xs
+      }
+      acr := {
+        s.acr with
+        keys := s.acr.keys.insert ⟨s.env.cta, x⟩
+        ref := ref'
+      }
+      env := s.env
+    }
+
+def Option.trace {ξ} [ToString ξ] : Option ξ → Option ξ
+  | none => none
+  | some x => dbg_trace x; some x
+
+
+-- match (dbg_trace "Gas left : {μ.gas}\n\nPC : {μ.pc}\nInst read : {i.toString}"; i) with
+-- w₀ : the 'checkpoint' world saved at the preparation stage of tx
+def exec (H : Block) (w₀ : World') : Nat → State' → Option exec.Result
+  | 0, _ => do (dbg_trace "NO INST\n"; none)
+  | lim + 1, s@⟨σ, μ, A, I⟩ => do
+    let i ← s.inst
+    match i with
+    | .next (.push bs _) => do
+       let g' ← safeSub μ.gas g_verylow
+       let m' : Machine := {
+         s.mcn with
+         gas := g'
+         pc := μ.pc + bs.length + 1
+         stk := (bs.toBits 32) :: s.mcn.stk
+       }
+       execAux s {s with mcn := m'} (exec H w₀ lim)
+    | .next (.reg .calldataload) => do
+      let (x :: xs) ← (return s.mcn.stk) | none
+      let g' ← s.deductGas g_verylow
+      let cd : Word := Bytes.toBits 32 (s.env.cld.sliceD x.toNat 32 0)
+      let s' := {s with mcn := {s.mcn with stk := cd :: xs, gas := g', pc := s.mcn.pc + 1}}
+      execAux s s' (exec H w₀ lim)
+    | .next (.reg .not) => do
+      let (x :: xs) ← (return s.mcn.stk) | none
+      let g' ← safeSub s.mcn.gas g_verylow
+      let s' := {s with mcn := {s.mcn with stk := x.not :: xs, gas := g', pc := s.mcn.pc + 1}}
+      execAux s s' (exec H w₀ lim)
+
+    | .next (.reg .add) => do
+      let (x :: y :: xs) ← (return s.mcn.stk) | none
+      let g' ← safeSub s.mcn.gas g_verylow
+      let s' := {s with mcn := {s.mcn with stk := (x + y) :: xs, gas := g', pc := s.mcn.pc + 1}}
+      execAux s s' (exec H w₀ lim)
+    | .next (.exec .call) => do
+      let (gas :: adr :: clv :: ilc :: isz :: olc :: osz :: stk)
+        ← (return s.mcn.stk) | none
+      let i : Bytes := s.mcn.mem.sliceD ilc.toNat isz.toNat 0
+      let t : Addr := toAddr adr
+      let acct ← s.wld.find? s.env.cta
+      let as' : AddrSet := s.acr.adrs.insert (toAddr adr)
+      let A' : Accrual := {s.acr with adrs := as'}
+
+
+      let cg : Nat := cCallGas s gas.toNat t clv
+
+      --let g' ← (dbg_trace "after EIP-2929 : "; (safeSub s.mcn.gas gColdAccountAccess).trace)
+      let g' ← safeSub s.mcn.gas gColdAccountAccess
+      --let g'' ← (dbg_trace "after deducting callgas : "; (safeSub g' cg).trace)
+      let g'' ← safeSub g' cg
+
+      let trState : State' :=
+         θ.prep H s.wld A' s.env.cta s.env.oga t t cg s.env.gpr.toNat clv clv i (s.env.exd - 1) s.env.wup
+      let trCore : theta.Result := θ.wrap trState (exec H w₀ lim trState)
+
+      let tr : theta.Result :=
+        if 0 < s.env.exd ∧ clv ≤ acct.bal
+        then trCore
+        else ⟨s.wld, cg, A', 0, []⟩
+      let cpy : Bytes := List.take osz.toNat tr.ret
+      let m' : Machine := {
+        gas := g'' + tr.gas
+        pc := s.mcn.pc + 1
+        mem := s.mcn.mem.takeD olc.toNat 0 ++ cpy ++ s.mcn.mem.drop (olc.toNat + cpy.length)
+        ret := tr.ret
+        stk := tr.sta :: stk
+      }
+
+      let s' : State' := {wld := tr.wld, mcn := m', acr := tr.acr, env := s.env}
+      let s'' : State' := s' -- todo : make s'' the result of deducting
+                             -- memory expansion gas costs from s'
+      execAux s s'' (exec H w₀ lim)
+    | .next (.reg .sstore) => do
+      let s' ← sstoreStep w₀ s
+      execAux s s' (exec H w₀ lim)
+    | .last .stop => some {wld := σ, mcn := μ, acr := A, ret := some []}
+    | _ => none
+
+def theta
+  (H : Block)
+  (σ₀ : World')
+  (σ : World')
+  (A : Accrual)
+  (s : Addr)
+  (o : Addr)
+  (r : Addr)
+  (c : Addr)
+  (g : Nat)
+  (p : Nat)
+  (v : Word)
+  (v_app : Word)
+  (d : Bytes)
+  (e : Nat)
+  (w : Bool) :
+  theta.Result :=
+  let xr := θ.prep H σ A s o r c g p v v_app d e w
+  θ.wrap xr (exec H σ₀ 100 xr)
+
+def foo :=
+  theta
+    testBlock
+    testCheckpoint
+    testCheckpoint
+    (A_star testBlock senderAdr (some receiverAdr) [])
+    senderAdr
+    senderAdr
+    receiverAdr
+    receiverAdr
+    g
+    10
+    1
+    1
+    testCallData
+    1024
+    true
+
+
+def g' : Nat := foo.gas
+
+def A_r : Nat := 0 -- SSTORE used only once, cannot change from 0
+
+def gstar : Nat := g' + min ((Tg - g') / 5) A_r
+
+def balInit : Nat := Bytes.toNat ((Hex.toBytes "0ba1a9ce0ba1a9ce").getD [])
+
+def txVal : Nat := 1
+
+-- def Yg : Nat := Tg - gstar
+def Yg : Nat := Tg - gstar
+
+def gasPrice : Nat := 10
+
+def balFinal : Nat := balInit - ((Yg * gasPrice) + txVal)
+
+#eval (Nat.toBytes balFinal).toHex
+#check Nat.toBytes
+
+
+def publicAddress (hsa : ByteArray) (ri : UInt8) (rsa : ByteArray) : IO Addr :=
+  match (ecrecoverFlag hsa ri rsa).toBytes with
+  | [] => IO.throw "Unreachable code : ecrecover should never return empty bytes"
+  | b :: pa =>
+    if b = 0
+    then IO.throw "ecrecover failed"
+    else return (Bytes.toBits 20 pa)
+
+def IO.guard (φ : Prop) [Decidable φ] (msg : String) : IO Unit :=
+  if φ then return () else IO.throw msg
+
+
+structure TxData : Type where
+  (nonce : Word)
+  (gasPrice : Word)
+  (gasLimit : Word)
+  (receiver : Addr)
+  (val : Word)
+  (calldata : Bytes)
+  (v : Byte)
+  (r : Bytes)
+  (s : Bytes)
+  (hash : Word)
+
+def decodeTxBytes (tbs : Bytes) : IO TxData := do
+  match RLP.decode tbs with
+  | RLP.list [
+      .bytes nonce,
+      .bytes gasPrice,
+      .bytes gasLimit,
+      .bytes toAddr,
+      .bytes val,
+      .bytes calldata,
+      .bytes [v],
+      .bytes r,
+      .bytes s
+    ] =>
+    let bs :=
+      RLP.encode <|
+        .list [
+          .bytes nonce,
+          .bytes gasPrice,
+          .bytes gasLimit,
+          .bytes toAddr,
+          .bytes val,
+          .bytes calldata
+        ]
+    return {
+      nonce := @Bytes.toBits 32 nonce
+      gasPrice := @Bytes.toBits 32 gasPrice
+      gasLimit := @Bytes.toBits 32 gasLimit
+      receiver := @Bytes.toBits 20 toAddr
+      val := @Bytes.toBits 32 val
+      calldata := calldata
+      v := v
+      r := r
+      s := s
+      hash := bs.keccak
+    }
+  | _ => IO.throw "Error : TX bytes decoding failed"
+
+def eqTest {ξ} [DecidableEq ξ] (x y : ξ) (testName : String) : IO Unit := do
+  .guard (x = y) (testName ++ " : fail")
+  .println (testName ++ " : pass")
+
+def main : IO Unit := do
+  let td ← readJsonFile "not.json" >>= Lean.Json.toTestData
+  IO.println td.toString
+  IO.println "======================================================"
+  let [t] ← getTests td | IO.throw "more than one test"
+  IO.println t.toString
+  let txd ← decodeTxBytes t.txdata
+
+  IO.println <| s!"v : {Bits.toHex 2 txd.v}"
+  IO.println <| s!"r : {txd.r.toHex}"
+  IO.println <| s!"s : {txd.s.toHex}"
+  IO.println <| s!"Hash of txdata excluding signature: {Bits.toHex 64 txd.hash}"
+
+  let rsa : ByteArray := Bytes.toBytesArray (txd.r ++ txd.s)
+  let hsa : ByteArray := Bytes.toBytesArray (@Bits.toBytes 32 txd.hash)
+  let ri : UInt8 := Byte.toUInt8 (txd.v - Ox x1 xB)
+
+  let sender ← publicAddress hsa ri rsa
+  IO.println <| s!"Recovered public address : {@Bits.toHex 40 sender}"
+
+  eqTest txd.nonce t.nonce "nonce check"
+  eqTest txd.gasPrice t.gasPrice "gas price check"
+  eqTest txd.gasLimit t.gasLimit "gas limit check"
+  eqTest sender t.sender "sender address check"
+  eqTest txd.receiver t.receiver "sender address check"
+  eqTest txd.val t.value "value check"
+  eqTest txd.calldata t.calldata "value check"
+
+
+  let g : Nat := txd.gasLimit.toNat - intrinsicGas (some txd.receiver) txd.calldata []
+
+  let blk : Block := {ben := t.coinbase}
+  let w ← (checkpoint t.world sender txd.val).toIO ""
+
+  let tr : theta.Result :=
+    theta
+      blk
+      w w
+      (A_star blk sender (some txd.receiver) [])
+      sender
+      sender
+      txd.receiver
+      txd.receiver
+      g
+      txd.gasPrice.toNat
+      txd.val
+      txd.val
+      txd.calldata
+      1024
+      true
+
+  let gasLeft : Nat := tr.gas
+  let refundAmount : Nat := 0 -- SSTORE used only once, cannot change from 0
+  let gasReturn : Nat := gasLeft + min ((Tg - g') / 5) refundAmount
+  let gasDiff : Nat := txd.gasLimit.toNat - gasReturn
+  let senderAcct ← (w.find? sender).toIO ""
+  let newBal : Nat := senderAcct.bal.toNat - (gasDiff * txd.gasPrice.toNat)
+
+  let newBalWord : Word := Nat.toBits' 256 newBal
+
+  IO.println s!"New sender balance : {@Bits.toHex 64 newBalWord}"
+
+  return ()
 
 
 #exit
 
+-- def main : IO Unit := do
+--   let td ← readJsonFile "not.json" >>= Lean.Json.toTestData
+--   IO.println td.toString
+
+-- def main : IO Unit := IO.println WethByteCode
+-- def main : IO Unit := do IO.println <| Bits.toHex 64 (trie testNTB)
 
 def main : IO Unit := do
   let bs := notTxBytes
   let (RLP.list [nonce, gasPrice, gasLimit, toAddr, val, calldata, .bytes [v], .bytes r, .bytes s])
-    ← (Option.toIO <| RLP.decode bs)
+    ← (Option.toIO <| RLP.decode bs) ""
     | throw (IO.Error.userError "Error : RLP decoding failed")
-  let bs' := RLP.encode <| .list [txType, nonce, gasPrice, toAddr, val, calldata]
+  let bs' := RLP.encode <| .list [nonce, gasPrice, gasLimit, toAddr, val, calldata]
   let hs := bs'.keccak
 
   IO.println <| s!"v : {Bits.toHex 2 v}"
@@ -874,3 +1564,131 @@ def main : IO Unit := do
     if b = 0
     then IO.println "ecrecover failed"
     else IO.println <| s!"Recovered public address : {Bytes.toHex pa}"
+
+
+-- mutual
+--
+--   def Ξ
+--     (σ : World')
+--     (g : Nat)
+--     (A : Accrual)
+--     (I : Env) :
+--     Ξ.Result :=
+--   let μ : Machine := {gas := g, pc := 0, mem := [], ret := [], stk := []}
+--   let xr : exec.Result := (execCore ⟨σ, μ, A, I⟩).getD ⟨none, μ, A, none⟩
+--   {wld := xr.wld, gas := xr.mcn.gas, acr := xr.acr, ret := xr.ret}
+--
+--
+--   def θ
+--     (lim : Measure)
+--     (σ : World')
+--     (A : Accrual)
+--     (s : Addr)
+--     (o : Addr)
+--     (r : Addr)
+--     (c : Addr)
+--     (g : Nat)
+--     (p : Nat)
+--     (v : Word)
+--     (v_app : Word)
+--     (d : Bytes)
+--     (e : Nat)
+--     (w : Bool) :
+--     theta.Result :=
+--   let σ'₁ : World' :=
+--     match σ.find? r with
+--     | none =>
+--       if v = 0
+--       then σ
+--       else σ.insert r {nonce := 0, bal := v, stor := .empty, code := []}
+--     | some aᵣ => σ.insert r {aᵣ with bal := aᵣ.bal + v}
+--   let σ₁ : World' :=
+--     match σ'₁.find? s with
+--     | none =>
+--       if v = 0
+--       then σ'₁
+--       else (dbg_trace "unreachable code : nonzero value calls from empty accounts should never happen" ; σ'₁)
+--     | some aₛ => σ.insert s {aₛ with bal := aₛ.bal - v}
+--   let cd : Bytes := σ.code c
+--   let I : Env := {
+--     cta := r, oga := o, gpr := @Nat.toBits 256 p, cld := d
+--     cla := s, clv := v_app, code := cd, exd := e, wup := w
+--   }
+--   let Ξr : Ξ.Result :=
+--     match c.toNat with
+--     | 1 => (dbg_trace "unimplemented : precompiled contract"; sorry)
+--     | 2 => (dbg_trace "unimplemented : precompiled contract"; sorry)
+--     | 3 => (dbg_trace "unimplemented : precompiled contract"; sorry)
+--     | 4 => (dbg_trace "unimplemented : precompiled contract"; sorry)
+--     | 5 => (dbg_trace "unimplemented : precompiled contract"; sorry)
+--     | 6 => (dbg_trace "unimplemented : precompiled contract"; sorry)
+--     | 7 => (dbg_trace "unimplemented : precompiled contract"; sorry)
+--     | 8 => (dbg_trace "unimplemented : precompiled contract"; sorry)
+--     | 9 => (dbg_trace "unimplemented : precompiled contract"; sorry)
+--     | _ => Ξ lim σ₁ g A I
+--
+--   let σ_stars : Option World' := Ξr.wld
+--   let g_stars : Nat := Ξr.gas
+--   let A_stars : Accrual := Ξr.acr
+--   let o : Option Bytes := Ξr.ret
+--
+--   let σ' : World' := σ_stars.getD σ
+--   let g' : Nat := if σ_stars.isNone ∧ o.isNone then 0 else g_stars
+--   let A' : Accrual := if σ_stars.isNone then A else A_stars
+--   let z : Word := if σ_stars.isNone then 0 else 1
+--   -- o' is not from YP, but necessary to cast from 'Option Bytes' to 'Bytes'
+--   let o' : Bytes := o.getD []
+--   ⟨σ', g', A', z, o'⟩
+--   termination_by lim
+--
+--   -- if EVM is in EHS at the point of running the Xinst, return 'none'.
+--   -- in all other cases, return 'some'
+--   def Xinst.run (lim : Measure) (s : State') : Xinst → Option State'
+--     | .call => do
+--       let (gas :: adr :: clv :: ilc :: isz :: olc :: osz :: stk)
+--         ← (return s.mcn.stk) | none
+--       let i : Bytes := s.mcn.mem.sliceD ilc.toNat isz.toNat 0
+--       let t : Addr := toAddr adr
+--       let acct ← s.wld.find? s.env.cta
+--       let as' : AddrSet := s.acr.adrs.insert (toAddr adr)
+--       let A' : Accrual := {s.acr with adrs := as'}
+--       let cg : Nat := cCallGas s gas.toNat t clv
+--       let tr : theta.Result :=
+--         if 0 < s.env.exd ∧ clv ≤ acct.bal
+--         then θ lim s.wld A' s.env.cta s.env.oga t t cg
+--                s.env.gpr.toNat clv clv i (s.env.exd - 1) s.env.wup
+--         else ⟨s.wld, cg, A', 0, []⟩
+--       let cpy : Bytes := List.take osz.toNat tr.ret
+--       let m' : Machine := {
+--         gas := s.mcn.gas - cg + tr.gas
+--         pc := s.mcn.pc + 1
+--         mem := s.mcn.mem.takeD olc.toNat 0 ++ cpy ++ s.mcn.mem.drop (olc.toNat + cpy.length)
+--         ret := tr.ret
+--         stk := tr.sta :: s.mcn.stk
+--       }
+--       some {wld := tr.wld, mcn := m', acr := tr.acr, env := s.env}
+--     | _ => none
+--   termination_by lim
+--
+--   def Ninst.run (lim : Measure) (s : State') : Ninst → Option State'
+--     | .push bs _ => do
+--       let g' ← safeSub s.mcn.gas g_verylow
+--       return {s with mcn := {s.mcn with stk := (bs.toBits 32) :: s.mcn.stk, gas := g'}}
+--     | .exec x => x.run lim s
+--     | .reg r => r.run s
+--   termination_by lim
+--
+--   def execCore (lim : Measure) (s : State') : Option exec.Result :=
+--     match lim with
+--     | 0 => none
+--     | k + 1 =>  do
+--       let i ← s.inst
+--       match i with
+--       | .next n => n.run k s >>= execCore k --⟨k, false⟩
+--       | .jump j => none
+--       | .last l => none
+--   termination_by lim
+--
+  -- -- X of YP
+  -- def exec (s : State') : exec.Result :=
+  --   (execCore (s.mcn.gas + 1) s).getD ⟨none, s.mcn, s.acr, none⟩
